aarch64 refine: SMC caps
Similarly to AInvs in the previous commit, introduce an arch_capBadge
interface with corresponding lemmas since SMC caps have badges and use
the general badge mechanisms.

The previous assumption that arch caps do not have badges also comes out
in the is_arch_update' predicate which now needs to explicitly demand
that the cap badge is None. This actually simplifies some proofs in the
architecture dependent part, but needs minor updates in Orphanage.

Also move up the definition of arch_cap'_fun_lift and introduce an
abbreviation arch_cap'_pred that can be used to lift arch cap predicates
to all caps (returning False on generic caps).

Signed-off-by: Gerwin Klein <gerwin.klein@proofcraft.systems>

proof/refine/AARCH64/ArchStateRelation.thy
@@ -43,6 +43,8 @@ primrec acap_relation :: "arch_cap \<Rightarrow> arch_capability \<Rightarrow> b
         arch_capability.VCPUCap vcpu)"
 | "acap_relation (arch_cap.SGISignalCap irq target) c  = (c =
         arch_capability.SGISignalCap (ucast irq) (ucast target))"
+| "acap_relation (arch_cap.SMCCap smc_badge) c  = (c =
+        arch_capability.SMCCap smc_badge)"
 
 definition abs_asid_entry :: "asidpool_entry \<Rightarrow> asid_pool_entry" where
   "abs_asid_entry ap = AARCH64_A.ASIDPoolVSpace (apVMID ap) (apVSpace ap)"
